vol-1/assignements/repeat.v
@@ -12,7 +12,7 @@ Import ListNotations.
 From LF Require Import Imp.
 
 
-(* 
+(*
 
 Let's go back to the IMP language described in Imp.v
 
@@ -22,52 +22,57 @@ described by the following rules
 
   st =[ c ]=>  st'       beval st' b = true
 ------------------------------------------------ (E_Re_End)
-    st =[ REPEAT c UNTIL b END ] => st'  
+    st =[ REPEAT c UNTIL b END ] => st'
 
 
-   st =[ c ]=>  st'   beval st' b = false  st' =[ REPEAT c UNTIL b END ] => st''   
+   st =[ c ]=>  st'   beval st' b = false  st' =[ REPEAT c UNTIL b END ] => st''
 --------------------------------------------------------------------------------- (E_Re_Loop)
-                st =[ REPEAT c UNTIL b END ] => st''  
+                st =[ REPEAT c UNTIL b END ] => st''
 
 
 In fact, REPEAT does *not* need to be taken as primitive, but it can be
 *defined* in terms of the constructors of com.
 
-1.1. ***Define*** it in terms of the original language of com, using the 
+1.1. ***Define*** it in terms of the original language of com, using the
 While construct. Fill in the following definition:
  *)
 
  Module RepeatDefined.
- 
-   
- Definition REP  (c : com) (b : bexp) : com.				     
-(* your definition here *)
- 
+
+
+Definition REP  (c : com) (b : bexp) : com :=
+<{
+  c;
+  while (BNot b) do
+    c
+  end
+}>.
+
  (*
- 
+
  1.2. Introduce an appropriate Notation.
- 
+
  1.3. Prove the above rules E_Re_End and E_Re_Loop are *derived*
  rules. That is, they do not need to be defined inductively but just
  stated and proven as Theorems, with respect to the original ceval
  relation.
 
  Again, do NOT redefine ceval.
-  
+
  1.4 State and prove the inversion principle for the construct, that
  is a Theorem like:
- 
+
  forall b c st st', st =[(REPEAT c UNTIL b END) => st' implies that
  either b is true in st and st=[ c] => st' or there exists a st'' such
  that ....
- 
+
  This theorem makes explicit the reasoning behind the inversion tactic
    and corresponds to reading the two above rules from the bottom
    up. It can be proven directly via inversion w/o any auxiliary
    lemmas.  *)
- 
- 
+
+
  End RepeatDefined.
- 
+
 
 
